src/Comparse.Parser.Builtins.fsti
@@ -4,85 +4,40 @@ open Comparse.Bytes.Typeclass
 open Comparse.Tactic.Attributes
 open Comparse.Utils
 
-(*** Basic definitions ***)
+(*** Type definitions ***)
 
-let rec for_allP (#a:Type) (pre:a -> prop) (l:list a): prop =
-    match l with
-    | [] -> True
-    | h::t -> pre h /\ for_allP pre t
+/// This structure defines message format on a type.
+/// This is the one a user want to use: it's just parsing and serialization functions,
+/// with lemmas proving they are inverse of each other.
+/// It means that we can't accidentally produce "bad" parsers or serializers:
+/// instances of this type ar guaranteed to be correct.
 
-val for_allP_eq: #a:Type -> pre:(a -> prop) -> l:list a ->
-  Lemma (for_allP pre l <==> (forall x. List.Tot.memP x l ==> pre x))
+noeq type parser_serializer_whole (bytes:Type0) {|bytes_like bytes|} (a:Type) = {
+  parse: bytes -> option a;
+  serialize: a -> bytes;
+  parse_serialize_inv: x:a -> Lemma (
+    parse (serialize x) == Some x
+  );
+  serialize_parse_inv: buf:bytes -> Lemma (
+    match parse buf with
+    | Some x -> serialize x == buf
+    | None -> True
+  );
+}
 
 ///   add_prefixes [prefix0; prefix1; ...; prefixn] suffix
 /// = concat prefix0 (concat prefix1 (... (concat prefixn suffix)))`
 let add_prefixes (#bytes:Type) {|bytes_like bytes|} (prefixes:list bytes) (suffix:bytes): bytes =
   List.Tot.fold_right (concat #bytes) prefixes suffix
 
-[@@"opaque_to_smt"]
-let prefixes_length (#bytes:Type) {|bytes_like bytes|} (l:list bytes) =
-  let add (x:nat) (y:nat): nat = x+y in
-  List.Tot.fold_right add (List.Tot.map length l) 0
-
-/// The following structure defines composable parsers / serializer.
+/// The following structure defines non-extensible message format on a type.
+/// It is useful to be composed with combinators, such as the dependent pair combinator (`bind`).
 /// For a structure that is meant to actually be used by the user, see `parser_serializer_whole`.
 ///
-/// The parser takes as input a `bytes`, and returns an `option` (it can fail on malformed inputs) of an `a` (the parsed value) and a `bytes` (the suffix of the input that was not parsed).
-/// The serializer takes as input an `a`, and returns a list of `bytes`, that you need to concatenate with `add_prefixes`.
-///
-/// -- Begin parenthesis about symbolic bytes --
-///
-/// Why do we have to concatenate the bytes ourselve, can't the serializer do it itself?
-/// See the following example, using a C-like syntax:
-/// struct A {
-///   int a0;
-///   int a1;
-/// };
-/// struct B {
-///   int b0;
-///   int b1;
-/// };
-/// struct C {
-///   A a;
-///   B b;
-/// };
-/// If the serializer did the concatenations, where it what would happen:
-///   serialize_C c
-/// = serialize_A c.a + serialize_B c.b
-/// = (serialize_int c.a.a0 + serialize_int c.a.a1) + (serialize_int c.b.b0 + serialize_int c.b.b1)
-/// = (int_to_bytes  c.a.a0 + int_to_bytes  c.a.a1) + (int_to_bytes  c.b.b0 + int_to_bytes  c.b.b1)
-///
-/// When the serializer instead returns a list, you get:
-///   serialize_C c
-/// = serialize_A c.a @ serialize_B c.b
-/// = (serialize_int c.a.a0  @ serialize_int c.a.a1 ) @ (serialize_int c.b.b0  @ serialize_int c.b.b1 )
-/// = ([int_to_bytes c.a.a0] @ [int_to_bytes c.a.a1]) @ ([int_to_bytes c.b.b0] @ [int_to_bytes c.b.b1])
-/// = [ int_to_bytes c.a.a0;    int_to_bytes c.a.a1;      int_to_bytes c.b.b0;    int_to_bytes c.b.b1]
-/// Hence `add_prefixes (serialize_C c) empty` is equal to:
-/// = int_to_bytes c.a.a0 + (int_to_bytes c.a.a1 + (int_to_bytes c.b.b0 + (int_to_bytes c.b.b1 + empty)))
-///
-/// Note how the parenthesing changes!
-/// On concrete bytes, this is equivalent. However, on symbolic bytes, we don't have associativity of concatenation.
-/// In the symbolic world, if you want to slice `a + b`, then the slice would only work in one of the following cases:
-/// - slice from `0` to `length a` to get `a`
-/// - slice from `length a` to `length (a+b)` to get `b`
-/// It means that in (a + b) + c`, you can't get `a` in one slice, you have to do it in two steps:
-/// - slice to obtain `a+b`
-/// - slice to obtain `a`
-///
-/// The last parenthesing is better for parsing, because parsing is done in the following order:
-/// - parse a0
-/// - parse a1
-/// - construct a = A{a0; a1}
-/// - parse b0
-/// - parse b1
-/// - construct b = B{b0; b1}
-/// - construct c = C{a; b}
-/// In the first parenthesing, the parser would need to guess the size of the structure A.
-/// In this example, this would be possible, however in the general case A could e.g. contain a variable-length list.
-/// In the last parenthesing, the parser would work fine with symbolic bytes.
-///
-/// -- End parenthesis about symbolic bytes --
+/// With non-extensible message formats, on every `bytes`, there is at most one prefix that is parseable.
+/// The `parse` function find this prefix and parses it.
+/// It returns an `option` (it can fail on malformed inputs) of an `a` (the parsed value) and a `bytes` (the suffix of the input that was not parsed).
+/// The serializer takes as input an `a`, and returns a list of `bytes`, that you need to concatenate with `add_prefixes` (see parenthesis just after the type definition).
 ///
 /// The parser and serializer are inverse of each other, as stated by the `..._inv` lemmas.
 
@@ -99,9 +54,105 @@ noeq type parser_serializer_prefix (bytes:Type0) {|bytes_like bytes|} (a:Type) =
   );
 }
 
+/// -- Begin parenthesis about symbolic bytes --
+///
+/// Why do we have to concatenate the bytes ourselve, can't the serializer do it itself?
+/// See the following example, using a C-like syntax:
+/// struct A {
+///   int x;
+///   int y;
+/// };
+/// struct B {
+///   int z;
+///   int w;
+/// };
+/// struct C {
+///   A a;
+///   B b;
+/// };
+/// If the serializer did the concatenations, where it what would happen:
+///   serialize_C c
+/// = serialize_A c.a + serialize_B c.b
+/// = (serialize_int c.a.x + serialize_int c.a.y) + (serialize_int c.b.z + serialize_int c.b.w)
+/// = (int_to_bytes  c.a.x + int_to_bytes  c.a.y) + (int_to_bytes  c.b.z + int_to_bytes  c.b.w)
+///
+/// When the serializer instead returns a list, you get:
+///   serialize_C c
+/// = serialize_A c.a @ serialize_B c.b
+/// = (serialize_int c.a.x  @ serialize_int c.a.y ) @ (serialize_int c.b.z  @ serialize_int c.b.w )
+/// = ([int_to_bytes c.a.x] @ [int_to_bytes c.a.y]) @ ([int_to_bytes c.b.z] @ [int_to_bytes c.b.w])
+/// = [ int_to_bytes c.a.x;    int_to_bytes c.a.y;      int_to_bytes c.b.z;    int_to_bytes c.b.w]
+/// Hence `add_prefixes (serialize_C c) empty` is equal to:
+/// = int_to_bytes c.a.x + (int_to_bytes c.a.y + (int_to_bytes c.b.z + (int_to_bytes c.b.w + empty)))
+///
+/// Note how the parenthesing changes!
+/// On concrete bytes, this is equivalent. However, on symbolic bytes, we don't necessarily have associativity of concatenation.
+/// In the symbolic world, if you want to slice `a + b`, then the slice would only work in one of the following cases:
+/// - slice from `0` to `length a` to get `a`
+/// - slice from `length a` to `length (a+b)` to get `b`
+/// It means that in (a + b) + c`, you can't get `a` in one slice, you have to do it in two steps:
+/// - slice to obtain `a+b`
+/// - slice to obtain `a`
+///
+/// The last parenthesing is better for parsing, because parsing is done in the following order:
+/// - parse x
+/// - parse y
+/// - construct a = A{x; y}
+/// - parse z
+/// - parse w
+/// - construct b = B{z; w}
+/// - construct c = C{a; b}
+/// In the first parenthesing, the parser would need to guess the size of the structure A.
+/// In this example, this would be possible, however in the general case A could e.g. contain a variable-length list.
+/// In the last parenthesing, the parser would work fine with symbolic bytes.
+///
+/// -- End parenthesis about symbolic bytes --
+
+let rec for_allP (#a:Type) (pre:a -> prop) (l:list a): prop =
+    match l with
+    | [] -> True
+    | h::t -> pre h /\ for_allP pre t
+
+val for_allP_eq: #a:Type -> pre:(a -> prop) -> l:list a ->
+  Lemma (for_allP pre l <==> (forall x. List.Tot.memP x l ==> pre x))
+
+[@@"opaque_to_smt"]
+let prefixes_length (#bytes:Type) {|bytes_like bytes|} (l:list bytes) =
+  let add (x:nat) (y:nat): nat = x+y in
+  List.Tot.fold_right add (List.Tot.map length l) 0
+
+/// `is_not_unit` is a predicate that detects message formats that have the non-emptiness property.
+/// In some combinators (such as the list combinator, `ps_whole_list`),
+/// it is useful to know that `parse` will never consume 0 bytes.
+/// Such types only have one element, hence are isomorphic to `unit`.
+///
+/// We include it as a separate predicate, and do not enforce this property in `parser_serializer_prefix`
+/// because it useful for example to define the formatting of `optional`:
+///   struct {
+///       uint8 present;
+///       select (present) {
+///           case 0: struct{}; //<-- parsed with ps_unit!
+///           case 1: T value;
+///       }
+///   } optional<T>;
+
+val is_not_unit: #bytes:Type0 -> {|bytes_like bytes|} -> #a:Type -> ps_a:parser_serializer_prefix bytes a -> Type0
+
+/// We define a special type for message formats with non-extensibility and non-emptiness,
+/// because they are the most common ones we encounter in the wild.
+/// The type `parser_serializer` will be the one most often used by the user,
+/// hence this nice name instead of something like `parser_serializer_prefix_not_unit`
+/// In this file, we tried to use `parser_serializer` for return types when possible,
+/// and to use `parser_serializer_prefix` for argument types when possible.
+
+let parser_serializer (bytes:Type0) {|bytes_like bytes|} (a:Type) = ps_a:parser_serializer_prefix bytes a{is_not_unit ps_a}
+
 /// Predicate transformer `is_well_formed`:
 /// given a predicate on `bytes` compatible with `concat` and `slice`, you get a predicate on `a`,
 /// which says whether the bytes predicate is valid on all the bytes contained inside `a`.
+
+let is_well_formed_whole (#bytes:Type0) {|bytes_like bytes|} (#a:Type) (ps_a:parser_serializer_whole bytes a) (pre:bytes_compatible_pre bytes) (x:a) =
+  pre (ps_a.serialize x)
 
 let is_well_formed_prefix (#bytes:Type0) {|bytes_like bytes|} (#a:Type) (ps_a:parser_serializer_prefix bytes a) (pre:bytes_compatible_pre bytes) (x:a) =
   for_allP pre (ps_a.serialize x)
@@ -115,32 +166,51 @@ val is_well_formed_prefix_weaken:
   (requires is_well_formed_prefix ps_a pre_strong x /\ (forall b. pre_strong b ==> pre_weak b))
   (ensures is_well_formed_prefix ps_a pre_weak x)
 
-/// What is the reason behind `parser_serializer_prefix` and `parser_serializer`?
-/// In some functions (such as `ps_whole_list` which is used to build `ps_seq` or `ps_bytes`),
-/// it is useful to know that `parse` will never consume 0 bytes, and `serialize` will never return `bytes_empty`.
-/// Such types only have one element, hence are isomorphic to `unit`. They are (anti-)recognized by the `is_not_unit` predicate.
-/// Thus they depend on a `parser_serializer` which doesn't serialize/parse a unit type.
-/// It is however very useful to be able to parse a unit type, in the example of an optional:
-///   struct {
-///       uint8 present;
-///       select (present) {
-///           case 0: struct{}; //<-- parsed with ps_unit!
-///           case 1: T value;
-///       }
-///   } optional<T>;
-/// In this interface, we tried to use `parser_serializer` for return types when possible,
-/// and to use `parser_serializer_prefix` for argument types when possible.
-/// The type `parser_serializer` will be the one most often used by the user,
-/// hence this nice name instead of something like `parser_serializer_prefix_not_unit`
+(*** Parser for basic types ***)
 
-val is_not_unit: #bytes:Type0 -> {|bytes_like bytes|} -> #a:Type -> ps_a:parser_serializer_prefix bytes a -> Type0
-let parser_serializer (bytes:Type0) {|bytes_like bytes|} (a:Type) = ps_a:parser_serializer_prefix bytes a{is_not_unit ps_a}
+[@@is_parser; is_parser_for (`%unit)]
+val ps_unit: #bytes:Type0 -> {| bytes_like bytes |} -> parser_serializer_prefix bytes unit
 
-(*** Parser combinators ***)
+val ps_unit_serialize:
+  #bytes:Type0 -> {|bytes_like bytes|} ->
+  x:unit ->
+  Lemma ((ps_unit #bytes).serialize x == [])
+  [SMTPat ((ps_unit #bytes).serialize x)]
+
+val ps_unit_is_well_formed:
+  #bytes:Type0 -> {| bl:bytes_like bytes |} ->
+  pre:bytes_compatible_pre bytes -> x:unit ->
+  Lemma (is_well_formed_prefix (ps_unit #bytes #bl) pre x <==> True)
+  [SMTPat (is_well_formed_prefix (ps_unit #bytes #bl) pre x)]
+
+val ps_unit_length:
+  #bytes:Type0 -> {| bl:bytes_like bytes |} ->
+  x:unit ->
+  Lemma (prefixes_length ((ps_unit #bytes #bl).serialize x) == 0)
+  [SMTPat (prefixes_length ((ps_unit #bytes #bl).serialize x))]
+
+val ps_whole_bytes:
+  #bytes:Type0 -> {|bytes_like bytes|} ->
+  parser_serializer_whole bytes bytes
+
+val ps_whole_bytes_serialize:
+  #bytes:Type0 -> {|bytes_like bytes|} ->
+  b:bytes ->
+  Lemma ((ps_whole_bytes #bytes).serialize b == b)
+  [SMTPat ((ps_whole_bytes #bytes).serialize b)]
+
+(*** Dependent pair combinator ***)
+(*** (non-extensible flavor) ***)
 
 /// A parser for dependant pairs.
 /// It can be used both to parse (non-dependant pairs), hence records,
 /// or tagged-union-like structures (the second value depend on the tag), hence sum types.
+///
+/// It is called `bind`, due to its similarity with the monadic bind:
+///   M a -> (  a -> M b    ) -> M        b
+/// versus
+///   M a -> (x:a -> M (b x)) -> M (x:a & b x)
+/// It can even be used as-is with F*'s do notation!
 
 val bind:
   #bytes:Type0 -> {|bytes_like bytes|} -> #a:Type -> #b:(a -> Type) ->
@@ -154,11 +224,11 @@ val bind_serialize:
   Lemma ((bind ps_a ps_b).serialize (|xa, xb|) == (ps_a.serialize xa) @ ((ps_b xa).serialize xb))
   [SMTPat ((bind ps_a ps_b).serialize (|xa, xb|))]
 
-/// On concrete bytes we actually have an equivalence between the `requires` and the `ensures`.
-/// On symbolic bytes where you may have multiple bytes of length 0, this is not true anymore.
-/// Hopefully, we only need this implication:
-/// the other would be useful to prove that a predicate do parse the unit type,
-/// and this is not something we actually need.
+// On concrete bytes we actually have an equivalence between the `requires` and the `ensures`.
+// On symbolic bytes where you may have multiple bytes of length 0, this is not true anymore.
+// Hopefully, we only need this implication:
+// the other would be useful to prove that a predicate do parse the unit type,
+// and this is not something we actually need.
 
 val bind_is_not_unit: #bytes:Type0 -> {| bytes_like bytes |} -> #a:Type -> #b:(a -> Type) -> ps_a:parser_serializer_prefix bytes a -> ps_b:(xa:a -> parser_serializer_prefix bytes (b xa)) -> Lemma
   (requires is_not_unit ps_a \/ (forall xa. is_not_unit (ps_b xa)))
@@ -184,6 +254,31 @@ val bind_length:
   xa:a -> xb:b xa ->
   Lemma (eq2 #nat (prefixes_length ((bind ps_a ps_b).serialize (|xa, xb|))) ((prefixes_length (ps_a.serialize xa)) + (prefixes_length ((ps_b xa).serialize xb))))
   [SMTPat (prefixes_length ((bind ps_a ps_b).serialize (|xa, xb|)))]
+
+(*** Dependent pair combinator ***)
+(*** (extensible flavor) ***)
+
+val bind_whole:
+  #bytes:Type0 -> {|bytes_like bytes|} -> #a:Type -> #b:(a -> Type) ->
+  ps_a:parser_serializer_prefix bytes a -> ps_b:(xa:a -> parser_serializer_whole bytes (b xa)) ->
+  parser_serializer_whole bytes (dtuple2 a b)
+
+val bind_whole_serialize:
+  #bytes:Type0 -> {|bytes_like bytes|} -> #a:Type -> #b:(a -> Type) ->
+  ps_a:parser_serializer_prefix bytes a -> ps_b:(xa:a -> parser_serializer_whole bytes (b xa)) ->
+  xa:a -> xb:b xa ->
+  Lemma ((bind_whole ps_a ps_b).serialize (|xa, xb|) == add_prefixes (ps_a.serialize xa) ((ps_b xa).serialize xb))
+  [SMTPat ((bind_whole ps_a ps_b).serialize (|xa, xb|))]
+
+val bind_whole_is_well_formed_whole:
+  #bytes:Type0 -> {| bytes_like bytes |} -> #a:Type -> #b:(a -> Type) ->
+  ps_a:parser_serializer_prefix bytes a -> ps_b:(xa:a -> parser_serializer_whole bytes (b xa)) ->
+  pre:bytes_compatible_pre bytes -> xa:a -> xb:(b xa) ->
+  Lemma (is_well_formed_whole (bind_whole ps_a ps_b) pre (|xa, xb|) <==> is_well_formed_prefix ps_a pre xa /\ is_well_formed_whole (ps_b xa) pre xb)
+  [SMTPat (is_well_formed_whole (bind_whole ps_a ps_b) pre (|xa, xb|))]
+
+(*** Isomorphism combinator ***)
+(*** (non-extensible flavor) ***)
 
 noeq type isomorphism_between (a:Type) (b:Type) = {
   a_to_b: a -> b;
@@ -262,7 +357,49 @@ val isomorphism_length:
   Lemma (prefixes_length ((isomorphism ps_a iso).serialize xb) == prefixes_length (ps_a.serialize (iso.b_to_a xb)))
   [SMTPat (prefixes_length ((isomorphism ps_a iso).serialize xb))]
 
+(*** Isomorphism combinator ***)
+(*** (extensible flavor) ***)
 
+val isomorphism_whole:
+  #bytes:Type0 -> {| bytes_like bytes |} -> #a:Type -> #b:Type ->
+  ps_a:parser_serializer_whole bytes a -> iso:isomorphism_between a b ->
+  parser_serializer_whole bytes b
+
+val isomorphism_whole_serialize:
+  #bytes:Type0 -> {| bytes_like bytes |} -> #a:Type -> #b:Type ->
+  ps_a:parser_serializer_whole bytes a -> iso:isomorphism_between a b ->
+  x:b ->
+  Lemma ((isomorphism_whole ps_a iso).serialize x == ps_a.serialize (iso.b_to_a x))
+  [SMTPat ((isomorphism_whole ps_a iso).serialize x)]
+
+val isomorphism_whole_is_well_formed:
+  #bytes:Type0 -> {| bytes_like bytes |} -> #a:Type -> #b:Type ->
+  ps_a:parser_serializer_whole bytes a -> iso:isomorphism_between a b ->
+  pre:bytes_compatible_pre bytes -> xb:b ->
+  Lemma
+  (is_well_formed_whole (isomorphism_whole ps_a iso) pre xb <==> is_well_formed_whole ps_a pre (iso.b_to_a xb))
+  [SMTPat (is_well_formed_whole (isomorphism_whole ps_a iso) pre xb)]
+
+let mk_isomorphism_whole
+  (#bytes:Type0) {| bytes_like bytes |} (#a:Type) (b:Type)
+  (ps_a:parser_serializer_whole bytes a) (a_to_b:a -> b) (b_to_a:b -> a):
+  Pure (parser_serializer_whole bytes b)
+    (requires (forall x. a_to_b (b_to_a x) == x) /\ (forall x. b_to_a (a_to_b x) == x))
+    (ensures fun _ -> True)
+  =
+  isomorphism_whole ps_a (mk_isomorphism_between a_to_b b_to_a)
+
+let mk_trivial_isomorphism_whole
+  (#bytes:Type0) {| bytes_like bytes |} (#a:Type) (#b:Type)
+  (ps_a:parser_serializer_whole bytes a):
+  Pure (parser_serializer_whole bytes b)
+    (requires a `subtype_of` b /\ b `subtype_of` a)
+    (ensures fun _ -> True)
+  =
+  isomorphism_whole ps_a ({a_to_b = (fun (x:a) -> (x <: b)); b_to_a = (fun (x:b) -> (x <: a)); a_to_b_to_a = (fun _ -> ()); b_to_a_to_b = (fun _ -> ()); })
+
+(*** Refinement combinator ***)
+(*** (non-extensible flavor) ***)
 
 // Introducing this type helps SMTPats to avoid dealing with the lambda `fun x -> pred x`
 type refined (a:Type) (pred:a -> bool) = x:a{pred x}
@@ -302,121 +439,8 @@ val refine_length:
   Lemma (prefixes_length ((refine ps_a pred).serialize x) == prefixes_length (ps_a.serialize x))
   [SMTPat (prefixes_length ((refine ps_a pred).serialize x))]
 
-(*** Parser for basic types ***)
-
-[@@is_parser; is_parser_for (`%unit)]
-val ps_unit: #bytes:Type0 -> {| bytes_like bytes |} -> parser_serializer_prefix bytes unit
-
-val ps_unit_serialize:
-  #bytes:Type0 -> {|bytes_like bytes|} ->
-  x:unit ->
-  Lemma ((ps_unit #bytes).serialize x == [])
-  [SMTPat ((ps_unit #bytes).serialize x)]
-
-val ps_unit_is_well_formed:
-  #bytes:Type0 -> {| bl:bytes_like bytes |} ->
-  pre:bytes_compatible_pre bytes -> x:unit ->
-  Lemma (is_well_formed_prefix (ps_unit #bytes #bl) pre x <==> True)
-  [SMTPat (is_well_formed_prefix (ps_unit #bytes #bl) pre x)]
-
-val ps_unit_length:
-  #bytes:Type0 -> {| bl:bytes_like bytes |} ->
-  x:unit ->
-  Lemma (prefixes_length ((ps_unit #bytes #bl).serialize x) == 0)
-  [SMTPat (prefixes_length ((ps_unit #bytes #bl).serialize x))]
-
-(*** Whole parsers ***)
-
-/// This structure describe the non-composable interface for parser
-/// The lemmas are similar (but simpler!) as the ones in `parser_serializer_prefix`
-///
-/// -- Begin parenthesis --
-///
-/// Actually, these parsers are useful for composability purposes.
-/// Here is how we construct a `parser_serializer (list a)` given a `parser_serializer a:
-///
-/// Step 1: use `ps_whole_list` to construct a `parser_serializer_whole (list a)` using `parser_serializer a`.
-/// This whole parser runs repeatedly the parser of a to the bytes, to construct a list of a.
-///
-/// Step 2: use `pse_to_ps` that first read a prefix containing the length, then slice the input bytes to have exactly the bytes containing the list and feed it to the whole parser.
-///
-/// -- End parenthesis --
-
-noeq type parser_serializer_whole (bytes:Type0) {|bytes_like bytes|} (a:Type) = {
-  parse: bytes -> option a;
-  serialize: a -> bytes;
-  parse_serialize_inv: x:a -> Lemma (
-    parse (serialize x) == Some x
-  );
-  serialize_parse_inv: buf:bytes -> Lemma (
-    match parse buf with
-    | Some x -> serialize x == buf
-    | None -> True
-  );
-}
-
-let is_well_formed_whole (#bytes:Type0) {|bytes_like bytes|} (#a:Type) (ps_a:parser_serializer_whole bytes a) (pre:bytes_compatible_pre bytes) (x:a) =
-  pre (ps_a.serialize x)
-
-val bind_whole:
-  #bytes:Type0 -> {|bytes_like bytes|} -> #a:Type -> #b:(a -> Type) ->
-  ps_a:parser_serializer_prefix bytes a -> ps_b:(xa:a -> parser_serializer_whole bytes (b xa)) ->
-  parser_serializer_whole bytes (dtuple2 a b)
-
-val bind_whole_serialize:
-  #bytes:Type0 -> {|bytes_like bytes|} -> #a:Type -> #b:(a -> Type) ->
-  ps_a:parser_serializer_prefix bytes a -> ps_b:(xa:a -> parser_serializer_whole bytes (b xa)) ->
-  xa:a -> xb:b xa ->
-  Lemma ((bind_whole ps_a ps_b).serialize (|xa, xb|) == add_prefixes (ps_a.serialize xa) ((ps_b xa).serialize xb))
-  [SMTPat ((bind_whole ps_a ps_b).serialize (|xa, xb|))]
-
-val bind_whole_is_well_formed_whole:
-  #bytes:Type0 -> {| bytes_like bytes |} -> #a:Type -> #b:(a -> Type) ->
-  ps_a:parser_serializer_prefix bytes a -> ps_b:(xa:a -> parser_serializer_whole bytes (b xa)) ->
-  pre:bytes_compatible_pre bytes -> xa:a -> xb:(b xa) ->
-  Lemma (is_well_formed_whole (bind_whole ps_a ps_b) pre (|xa, xb|) <==> is_well_formed_prefix ps_a pre xa /\ is_well_formed_whole (ps_b xa) pre xb)
-  [SMTPat (is_well_formed_whole (bind_whole ps_a ps_b) pre (|xa, xb|))]
-
-val isomorphism_whole:
-  #bytes:Type0 -> {| bytes_like bytes |} -> #a:Type -> #b:Type ->
-  ps_a:parser_serializer_whole bytes a -> iso:isomorphism_between a b ->
-  parser_serializer_whole bytes b
-
-val isomorphism_whole_serialize:
-  #bytes:Type0 -> {| bytes_like bytes |} -> #a:Type -> #b:Type ->
-  ps_a:parser_serializer_whole bytes a -> iso:isomorphism_between a b ->
-  x:b ->
-  Lemma ((isomorphism_whole ps_a iso).serialize x == ps_a.serialize (iso.b_to_a x))
-  [SMTPat ((isomorphism_whole ps_a iso).serialize x)]
-
-val isomorphism_whole_is_well_formed:
-  #bytes:Type0 -> {| bytes_like bytes |} -> #a:Type -> #b:Type ->
-  ps_a:parser_serializer_whole bytes a -> iso:isomorphism_between a b ->
-  pre:bytes_compatible_pre bytes -> xb:b ->
-  Lemma
-  (is_well_formed_whole (isomorphism_whole ps_a iso) pre xb <==> is_well_formed_whole ps_a pre (iso.b_to_a xb))
-  [SMTPat (is_well_formed_whole (isomorphism_whole ps_a iso) pre xb)]
-
-/// This helper function is extremely valuable to help F*'s type inference.
-/// Using it, F* is able to automatically deduce the type of `a`, which is often ugly.
-/// (This is in general why you use `isomorphism`: because you want to replace the ugly `a` with a nicer `b`)
-let mk_isomorphism_whole
-  (#bytes:Type0) {| bytes_like bytes |} (#a:Type) (b:Type)
-  (ps_a:parser_serializer_whole bytes a) (a_to_b:a -> b) (b_to_a:b -> a):
-  Pure (parser_serializer_whole bytes b)
-    (requires (forall x. a_to_b (b_to_a x) == x) /\ (forall x. b_to_a (a_to_b x) == x))
-    (ensures fun _ -> True)
-  =
-  isomorphism_whole ps_a (mk_isomorphism_between a_to_b b_to_a)
-
-let mk_trivial_isomorphism_whole
-  (#bytes:Type0) {| bytes_like bytes |} (#a:Type) (#b:Type)
-  (ps_a:parser_serializer_whole bytes a):
-  Pure (parser_serializer_whole bytes b)
-    (requires a `subtype_of` b /\ b `subtype_of` a)
-    (ensures fun _ -> True)
-  =
-  isomorphism_whole ps_a ({a_to_b = (fun (x:a) -> (x <: b)); b_to_a = (fun (x:b) -> (x <: a)); a_to_b_to_a = (fun _ -> ()); b_to_a_to_b = (fun _ -> ()); })
+(*** Refinement combinator ***)
+(*** (extensible flavor) ***)
 
 val refine_whole:
   #bytes:Type0 -> {|bytes_like bytes|} -> #a:Type ->
@@ -430,71 +454,12 @@ val refine_whole_serialize:
   Lemma ((refine_whole ps_a pred).serialize x == ps_a.serialize x)
   [SMTPat ((refine_whole ps_a pred).serialize x)]
 
-(*** Conversion between prefix and whole parsers ***)
+(*** List combinator ***)
 
-val ps_prefix_to_ps_whole:
-  #bytes:Type0 -> {|bytes_like bytes|} -> #a:Type ->
-  parser_serializer_prefix bytes a ->
-  parser_serializer_whole bytes a
-
-val ps_prefix_to_ps_whole_serialize:
-  #bytes:Type0 -> {|bytes_like bytes|} -> #a:Type ->
-  ps_a:parser_serializer_prefix bytes a ->
-  x:a ->
-  Lemma ((ps_prefix_to_ps_whole ps_a).serialize x == add_prefixes (ps_a.serialize x) empty)
-  [SMTPat ((ps_prefix_to_ps_whole ps_a).serialize x)]
-
-val ps_prefix_to_ps_whole_is_well_formed:
-  #bytes:Type0 -> {|bytes_like bytes|} -> #a:Type ->
-  ps_a:parser_serializer_prefix bytes a ->
-  pre:bytes_compatible_pre bytes -> x:a ->
-  Lemma (is_well_formed_whole (ps_prefix_to_ps_whole ps_a) pre x <==> is_well_formed_prefix ps_a pre x)
-  [SMTPat (is_well_formed_whole (ps_prefix_to_ps_whole ps_a) pre x)]
-
-val ps_prefix_to_ps_whole_length:
-  #bytes:Type0 -> {|bytes_like bytes|} -> #a:Type ->
-  ps_a:parser_serializer_prefix bytes a ->
-  x:a ->
-  Lemma (length ((ps_prefix_to_ps_whole ps_a).serialize x) == prefixes_length (ps_a.serialize x))
-  [SMTPat (length ((ps_prefix_to_ps_whole ps_a).serialize x))]
-
-let ps_whole_length_pred
-  (#bytes:Type0) {|bytes_like bytes|} (#a:Type)
-  (ps_a:parser_serializer_whole bytes a) (n:nat) (x:a)
-  : bool =
-  length (ps_a.serialize x) = n
-
-val ps_whole_to_bare_ps_prefix:
-  #bytes:Type0 -> {|bytes_like bytes|} -> #a:Type ->
-  len:nat -> ps_a:parser_serializer_whole bytes a{forall x. length (ps_a.serialize x) == len} ->
-  parser_serializer_prefix bytes a
-
-val ps_whole_to_bare_ps_prefix_serialize:
-  #bytes:Type0 -> {|bytes_like bytes|} -> #a:Type ->
-  len:nat -> ps_a:parser_serializer_whole bytes a{forall x. length (ps_a.serialize x) == len} ->
-  x:a ->
-  Lemma ((ps_whole_to_bare_ps_prefix len ps_a).serialize x == [ps_a.serialize x])
-  [SMTPat ((ps_whole_to_bare_ps_prefix len ps_a).serialize x)]
-
-val ps_whole_to_bare_ps_prefix_is_not_unit:
-  #bytes:Type0 -> {|bytes_like bytes|} -> #a:Type ->
-  len:nat -> ps_a:parser_serializer_whole bytes a{forall x. length (ps_a.serialize x) == len} ->
-  Lemma
-  (requires 1 <= len)
-  (ensures is_not_unit (ps_whole_to_bare_ps_prefix len ps_a))
-  [SMTPat (is_not_unit (ps_whole_to_bare_ps_prefix len ps_a))]
-
-(*** Whole parsers ***)
-
-val ps_whole_bytes:
-  #bytes:Type0 -> {|bytes_like bytes|} ->
-  parser_serializer_whole bytes bytes
-
-val ps_whole_bytes_serialize:
-  #bytes:Type0 -> {|bytes_like bytes|} ->
-  b:bytes ->
-  Lemma ((ps_whole_bytes #bytes).serialize b == b)
-  [SMTPat ((ps_whole_bytes #bytes).serialize b)]
+/// This list combinator apply repeatedly a message format `ps_a`,
+/// resulting in an extensible message format:
+/// for example, the serialization of [x;y] will be a prefix of the serialization of [x;y;z].
+/// It can be combined by a length-prefixing mechanism to transform it into a non-extensible message format.
 
 val ps_whole_list:
   #bytes:Type0 -> {|bytes_like bytes|} -> #a:Type ->
@@ -529,6 +494,11 @@ val ps_whole_list_length:
 
 (*** Another list combinator ***)
 
+/// This list combinator doesn't require any length-prefixing to have the non-extensibility property:
+/// it uses the fact that the last element of the list will satisfy some predicate,
+/// while the other elements of the list won't satisfy it.
+/// It is useful, for example to derive message formats for null-terminated strings.
+
 let pred_not (#a:Type) (pred:a -> bool) (x:a): bool =
   not (pred x)
 
@@ -539,6 +509,17 @@ val ps_list_until:
   #bytes:Type0 -> {|bytes_like bytes|} -> #a:Type ->
   parser_serializer bytes a -> pred:(a -> bool) ->
   parser_serializer bytes (list_until a pred)
+
+val ps_list_until_serialize:
+  #bytes:Type0 -> {|bytes_like bytes|} -> #a:Type ->
+  ps_a:parser_serializer bytes a -> pred:(a -> bool) ->
+  x:list_until a pred ->
+  Lemma
+  ((ps_list_until ps_a pred).serialize x == (
+    let (l, last) = x in
+    List.Tot.fold_right (@) (List.Tot.map ps_a.serialize l) (ps_a.serialize last)
+  ))
+  [SMTPat ((ps_list_until ps_a pred).serialize x)]
 
 val ps_list_until_is_well_formed:
   #bytes:Type0 -> {|bytes_like bytes|} -> #a:Type ->
@@ -551,3 +532,80 @@ val ps_list_until_is_well_formed:
     is_well_formed_prefix ps_a pre last
   ))
   [SMTPat (is_well_formed_prefix (ps_list_until ps_a pred) pre x)]
+
+val ps_list_until_length:
+  #bytes:Type0 -> {|bytes_like bytes|} -> #a:Type ->
+  ps_a:parser_serializer bytes a -> pred:(a -> bool) ->
+  x:list_until a pred ->
+  Lemma
+  (prefixes_length ((ps_list_until ps_a pred).serialize x) == (
+    let (l, last) = x in
+    bytes_length ps_a (List.Tot.map id l) +
+    prefixes_length (ps_a.serialize last)
+  ))
+  [SMTPat (prefixes_length ((ps_list_until ps_a pred).serialize x))]
+
+(*** Conversion from prefix to whole ***)
+
+/// This function "forgets" non-extensibility,
+/// and converts a `parser_serializer_prefix` to a `parser_serializer_whole`.
+/// One of its uses is to obtain a `parser_serializer_whole` which is more user-friendly.
+/// than `parser_serializer_prefix`, which is more an intermediate type (with stronger invariants).
+
+val ps_prefix_to_ps_whole:
+  #bytes:Type0 -> {|bytes_like bytes|} -> #a:Type ->
+  parser_serializer_prefix bytes a ->
+  parser_serializer_whole bytes a
+
+val ps_prefix_to_ps_whole_serialize:
+  #bytes:Type0 -> {|bytes_like bytes|} -> #a:Type ->
+  ps_a:parser_serializer_prefix bytes a ->
+  x:a ->
+  Lemma ((ps_prefix_to_ps_whole ps_a).serialize x == add_prefixes (ps_a.serialize x) empty)
+  [SMTPat ((ps_prefix_to_ps_whole ps_a).serialize x)]
+
+val ps_prefix_to_ps_whole_is_well_formed:
+  #bytes:Type0 -> {|bytes_like bytes|} -> #a:Type ->
+  ps_a:parser_serializer_prefix bytes a ->
+  pre:bytes_compatible_pre bytes -> x:a ->
+  Lemma (is_well_formed_whole (ps_prefix_to_ps_whole ps_a) pre x <==> is_well_formed_prefix ps_a pre x)
+  [SMTPat (is_well_formed_whole (ps_prefix_to_ps_whole ps_a) pre x)]
+
+val ps_prefix_to_ps_whole_length:
+  #bytes:Type0 -> {|bytes_like bytes|} -> #a:Type ->
+  ps_a:parser_serializer_prefix bytes a ->
+  x:a ->
+  Lemma (length ((ps_prefix_to_ps_whole ps_a).serialize x) == prefixes_length (ps_a.serialize x))
+  [SMTPat (length ((ps_prefix_to_ps_whole ps_a).serialize x))]
+
+(*** Conversion from whole to prefix ***)
+
+/// If a message format has fixed-length serialization, then it is non-extensible.
+/// This function is hence converts a `parser_serializer_whole` to a `parser_serializer_prefix`.
+
+let ps_whole_length_pred
+  (#bytes:Type0) {|bytes_like bytes|} (#a:Type)
+  (ps_a:parser_serializer_whole bytes a) (n:nat) (x:a)
+  : bool =
+  length (ps_a.serialize x) = n
+
+val ps_whole_to_bare_ps_prefix:
+  #bytes:Type0 -> {|bytes_like bytes|} -> #a:Type ->
+  len:nat -> ps_a:parser_serializer_whole bytes a{forall x. length (ps_a.serialize x) == len} ->
+  parser_serializer_prefix bytes a
+
+val ps_whole_to_bare_ps_prefix_serialize:
+  #bytes:Type0 -> {|bytes_like bytes|} -> #a:Type ->
+  len:nat -> ps_a:parser_serializer_whole bytes a{forall x. length (ps_a.serialize x) == len} ->
+  x:a ->
+  Lemma ((ps_whole_to_bare_ps_prefix len ps_a).serialize x == [ps_a.serialize x])
+  [SMTPat ((ps_whole_to_bare_ps_prefix len ps_a).serialize x)]
+
+val ps_whole_to_bare_ps_prefix_is_not_unit:
+  #bytes:Type0 -> {|bytes_like bytes|} -> #a:Type ->
+  len:nat -> ps_a:parser_serializer_whole bytes a{forall x. length (ps_a.serialize x) == len} ->
+  Lemma
+  (requires 1 <= len)
+  (ensures is_not_unit (ps_whole_to_bare_ps_prefix len ps_a))
+  [SMTPat (is_not_unit (ps_whole_to_bare_ps_prefix len ps_a))]
+
